specs

proofs/Challenge2_proof.v
@@ -16,3 +16,31 @@ Open Scope Z_scope.
 Hint Constructors LocallySorted.
 Hint Constructors Permutation.
 Ltac auto_tilde ::= try unfold LibListZ.length in *; rew_list in *; eauto with maths.
+
+Inductive color := R | B.
+Definition coloring := list color.
+
+(* Z_lt_le_dec: forall x y : int, {x < y} + {y <= x} *)
+
+Fixpoint coloring_valid (aux: int) (c : coloring) : bool :=
+  match c with
+  | B :: cs => if Z_lt_le_dec aux 3 then false else coloring_valid 0 cs
+  | R :: cs => coloring_valid (aux + 1) cs
+  | nil => if Z_lt_le_dec aux 3 then false else true
+  end.
+
+Definition invariant (n: int) (counts: list int) (colorings: list coloring) :=
+  length counts = n /\
+  length colorings = n /\
+  forall i, 0 <= i < n ->
+    counts[i] = length colorings[i] /\
+    Forall (fun c => length c = i) colorings.
+
+Lemma docount_spec : forall (a:loc) (L: list int),
+  app docount [count a]
+    PRE (a ~> Array L)
+    POST (fun (tt:unit) =>
+            Hexists L' C,
+            a ~> Array L' \* \[ invariant (length L') L' C ]).
+Proof.
+Admitted.
